\documentclass[a4paper]{book}
\usepackage{geometry}
% make full use of A4 papers
\geometry{margin=1.5cm, vmargin={0pt,1cm}}
\setlength{\topmargin}{-1cm}
\setlength{\paperheight}{29.7cm}
\setlength{\textheight}{25.1cm}

% auto adjust the marginals
\usepackage{marginfix}

\usepackage{amsfonts}
\usepackage{amsmath}
\usepackage{amssymb}
\usepackage{amsthm}
% \usepackage{CJKutf8}   % for Chinese characters
\usepackage{ctex}
\usepackage{enumerate}
\usepackage{graphicx}  % for figures
\usepackage{layout}
\usepackage{multicol}  % multiple columns to reduce number of pages
\usepackage{mathrsfs}
\usepackage{fancyhdr}
\usepackage{subfigure}
\usepackage{tcolorbox}
\usepackage{tikz-cd}
\usepackage{listings}
\usepackage{xcolor} %代码高亮
\usepackage{braket}
% ------------------
% common commands %
% ------------------
% differentiation
\newcommand{\gen}[1]{\left\langle#1 \right\rangle}
\newcommand{\dif}{\mathrm{d}}
\newcommand{\difPx}[1]{\frac{\partial#1}{\partial x}}
\newcommand{\difPy}[1]{\frac{\partial#1}{\partial y}}
\newcommand{\Dim}{\mathrm{D}}
\newcommand{\avg}[1]{\left\langle#1 \right\rangle}
\newcommand{\sgn}{\mathrm{sgn}}
\newcommand{\Span}{\mathrm{span}}
\newcommand{\dom}{\mathrm{dom}}
\newcommand{\Arity}{\mathrm{arity}}
\newcommand{\Int}{\mathrm{Int}}
\newcommand{\Ext}{\mathrm{Ext}}
\newcommand{\Cl}{\mathrm{Cl}}
\newcommand{\Fr}{\mathrm{Fr}}
% group is generated by
\newcommand{\grb}[1]{\left\langle#1 \right\rangle}
% rank
\newcommand{\rank}{\mathrm{rank}}
\newcommand{\Iden}{\mathrm{Id}}

% this environment is for solutions of examples and exercises
\newenvironment{solution}%
{\noindent\textbf{Solution.}}%
{\qedhere}
% the following command is for disabling environments
% so that their contents do not show up in the pdf.
\makeatletter
\newcommand{\voidenvironment}[1]{%
  \expandafter\providecommand\csname env@#1@save@env\endcsname{}%
  \expandafter\providecommand\csname env@#1@process\endcsname{}%
  \@ifundefined{#1}{}{\RenewEnviron{#1}{}}%
}
\makeatother

% ---------------------------------------------
% commands specifically for complex analysis %
% ---------------------------------------------
% complex conjugate
\newcommand{\ccg}[1]{\overline{#1}}
% the imaginary unit
\newcommand{\ii}{\mathbf{i}}
% \newcommand{\ii}{\boldsymbol{i}}
% the real part
\newcommand{\Rez}{\mathrm{Re}\,}
% the imaginary part
\newcommand{\Imz}{\mathrm{Im}\,}
% punctured complex plane
\newcommand{\pcp}{\mathbb{C}^{\bullet}}
% the principle branch of the logarithm
\newcommand{\Log}{\mathrm{Log}}
% the principle value of a nonzero complex number
\newcommand{\Arg}{\mathrm{Arg}}
\newcommand{\Null}{\mathrm{null}}
\newcommand{\Range}{\mathrm{range}}
\newcommand{\Ker}{\mathrm{ker}}
\newcommand{\Iso}{\mathrm{Iso}}
\newcommand{\Aut}{\mathrm{Aut}}
\newcommand{\ord}{\mathrm{ord}}
\newcommand{\Res}{\mathrm{Res}}
% \newcommand{\GL2R}{\mathrm{GL}(2,\mathbb{R})}
\newcommand{\GL}{\mathrm{GL}}
\newcommand{\SL}{\mathrm{SL}}
\newcommand{\Dist}[2]{\left|{#1}-{#2}\right|}

\newcommand\tbbint{{-\mkern-16mu\int}}
\newcommand\tbint{{\mathchar'26 -\mkern-14mu\int}}
\newcommand\dbbint{{-\mkern-20mu\int}}
\newcommand\dbint{{\mathchar'26 -\mkern-26mu\int}}
\newcommand\bint{
  {\mathchoice{\dbint}{\tbint}{\tbint}{\tbint}}
}
\newcommand\bbint{
  {\mathchoice{\dbbint}{\tbbint}{\tbbint}{\tbbint}}
}





% ----------------------------------------
% theorem and theorem-like environments %
% ----------------------------------------
\numberwithin{equation}{chapter}
\theoremstyle{definition}

\newtheorem{thm}{Theorem}[chapter]
\newtheorem{axm}[thm]{Axiom}
\newtheorem{alg}[thm]{Algorithm}
\newtheorem{asm}[thm]{Assumption}
\newtheorem{defn}[thm]{Definition}
\newtheorem{prop}[thm]{Proposition}
\newtheorem{rul}[thm]{Rule}
\newtheorem{coro}[thm]{Corollary}
\newtheorem{lem}[thm]{Lemma}
\newtheorem{exm}{Example}[chapter]
\newtheorem{rem}{Remark}[chapter]
\newtheorem{exc}[exm]{Exercise}
\newtheorem{frm}[thm]{Formula}
\newtheorem{ntn}{Notation}

% for complying with the convention in the textbook
\newtheorem{rmk}[thm]{Remark}


% \lstset{
%	backgroundcolor=\color{red!50!green!50!blue!50},%代码块背景色为浅灰色
%	rulesepcolor= \color{gray}, %代码块边框颜色
%	breaklines=true,  %代码过长则换行
%	numbers=left, %行号在左侧显示
%	numberstyle= \small,%行号字体
%	keywordstyle= \color{blue},%关键字颜色
%	commentstyle=\color{gray}, %注释颜色
%	frame=shadowbox%用方框框住代码块
% }
\lstset{
  columns=fixed,
  numbers=left,                                        % 在左侧显示行号
  numberstyle=\tiny\color{gray},                       % 设定行号格式
  frame=none,                                          % 不显示背景边框
  backgroundcolor=\color[RGB]{245,245,244},            % 设定背景颜色
  keywordstyle=\color[RGB]{40,40,255},                 % 设定关键字颜色
  numberstyle=\footnotesize\color{darkgray},
  commentstyle=\it\color[RGB]{0,96,96},                % 设置代码注释的格式
  stringstyle=\rmfamily\slshape\color[RGB]{128,0,0},   % 设置字符串格式
  showstringspaces=false,                              % 不显示字符串中的空格
  language=c++,                                        % 设置语言
}

% ----------------------
% the end of preamble %
% ----------------------

\begin{document}
\pagestyle{empty}
\pagenumbering{roman}
% 
% \tableofcontents
% \clearpage

% \pagestyle{fancy}
% \fancyhead{}
% \lhead{Qinghai Zhang}
% \chead{Notes on Algebraic Topology}
% \rhead{Fall 2018}


\setcounter{chapter}{4}
\pagenumbering{arabic}
% \setcounter{page}{0}

% --------------------------------------------------------
% uncomment the following to remove these environments
% to generate handouts for students.
% --------------------------------------------------------
% \begingroup
% \voidenvironment{rem}%
% \voidenvironment{proof}%
% \voidenvironment{solution}%


% each chapter is factored into a separate file.

\chapter{Homework 21935004 谭焱}
% \begin{lstlisting}
%   int main(){
%   double d;
%   int i;
%   return i;
% }
% \end{lstlisting}
% The main ingredients of snacks are sugar and fat;
% the main ingredients of math are logic and set theory.


\begin{multicols}{2}
  \setlength{\columnseprule}{0.2pt}

  \begin{exc}
    18.  (Stokes's rule) Assume $ u $ solves the initial-value problem
    \begin{equation}\label{eq:1}
    \begin{cases}
      \begin{aligned}
        u_{tt} - \Delta u = 0 \qquad &\textmd{in} \ \mathbb{R}^n \times (0, \infty) \\
        u = 0, \ u_t = h \qquad     &\textmd{on} \ \mathbb{R}^n \times \{t = 0\}.
      \end{aligned}
    \end{cases}
  \end{equation}
  Show that $v := u_t $ solves
  \begin{align}\label{eq:2}
    \begin{cases}
      v_{tt} - \Delta v = 0  \qquad & \textmd{in} \ \mathbb{R}^n \times (0, \infty)  \\
      v = h, \ v_t = 0 \qquad      & \textmd{on} \ \mathbb{R}^n \times \{t = 0\},
    \end{cases}
  \end{align}
  This is \textit{Stokes's rule}.
\end{exc}

\begin{solution}
  From (\ref{eq:1}) $v = u_t = h, \ v_t = {(u_t)}_t = h_t = 0$, since $h$ is constant for variable \textit{t}. \textit{u} solves the wave equation. Thus $h \in C^2(\mathbb{R}^n)$, and
  \begin{align*}
    v_{tt} - \Delta v =& {(u_t)}_{tt} - \Delta u_t \\
    =& {(u_{tt})}_t - {(\Delta u)}_t \\
    =& {(u_{tt} - \Delta u)}_t \\
    =& 0_t \\
    =& 0.
  \end{align*}
  So \textit{v} solves (\ref{eq:2}).
\end{solution}



\begin{exc}
  19.  
  \begin{enumerate} [(a)]
  \item Show the general solution of the \textbf{PDE} $u_{xy} = 0$ is
    \begin{equation*}
      u(x,y) = F(x) + G(y)
    \end{equation*}
    for arbitrary functions $F,G$.
  \item Using th changed of variables $\xi = x + t, \eta = x - t$, show $u_{tt} - u_{xx} = 0$ if and only if $u_{\xi \eta} = 0$.

  \item Use (a) and (b) to rederive d'Alembert's formula.

  \item Under what conditions on the initial data $g,h$ is the solution $u$ a right-moving wave? A left-moving wave?
    
  \end{enumerate}.
\end{exc}

\begin{solution}
  \begin{enumerate}[(a)]
  \item $u_{xy} = 0\ \Longleftrightarrow u_x = f(x)\ \Longleftrightarrow u = \int f(x)dx + g(y)$. Let $F(x) = \int f dx, \ G(y) = g(y)$ replace above get $u(x,y) = F(x) + G(y)$.

  \item $u_{tt} - u_{xx} = 0\ \Longleftrightarrow (\partial^2_t - \partial^2_x)(u) = 0\ \Longleftrightarrow (\partial_t + \partial_x)(\partial_t - \partial_x)(u) = 0 \ \Longleftrightarrow -\partial_{\xi} \partial_\eta (u) = 0 \Longleftrightarrow u_{\xi \eta} = 0$.

  \item From (a) and (b) we know the wave equation general solution is $u(x,t) = F(x+t) + G(x-t)$. Combining with inital condition
    \begin{align*}
      \begin{cases}
        F(x) + G(x) = g(x)   \\
        F_t(x) - G_t(x) = h(x).
      \end{cases}
    \end{align*}
    Solving the equations get $u(x,t) = \frac{1}{2}(g(x+t) + g(x-t)) + \int_{x-t}^{x+t} h(y) dy$.

    \item $F(x)$ is left-moving wave, since when \textit{t} increasing, \textit{x = -t} move left so that $F(x+t)$ maintain constant. Similarly, $G(y)$ is right-moving wave.
  \end{enumerate}
\end{solution}

\begin{exc}
  20.
  Assume that for some attenuation function $\alpha = \alpha(r) $ and delay function $\beta = \beta(r) \geq 0$, there eixst for \textit{all} profiles $\phi$ solutions of the wave equation in $(\mathbb{R}^n - {0}) \times \mathbb{R}$ having the form
  \begin{equation}
    \label{eq:3}
    u(x,t) = \alpha(t) \phi(r - \beta(r)).
  \end{equation}
  Here $r = |x|$ and we assume $\beta(0) = 0$.

  Show that this is possible only if $n = 1$ or 3, and compute the form of the functions $\alpha , \beta$.
\end{exc}

\begin{solution}
  Since $\partial_{x_i} r = \frac{x_i}{r} \ \Longrightarrow \Delta r = \frac{n-1}{r}$. Replacing the wave equation with (\ref{eq:3})
  \begin{align*}
    &\Delta(\alpha(r) \phi (t - \beta(r))) - \partial_t^2(\alpha(r) \phi(t - \beta(r))) = 0 \Longleftrightarrow \\
    &\alpha^{\prime \prime} \phi + \alpha \phi^{\prime \prime} ({(\beta^\prime)}^2 - 1) - 2\alpha^\prime\phi^{\prime} \beta^\prime +\\ &\frac{n-1}{r}(\alpha^\prime \phi - \alpha \phi^\prime \beta^\prime) - \alpha \phi^\prime \beta^{\prime \prime} = 0.
  \end{align*}
  It's true for every $\phi$ means that $\phi, \phi^\prime \textmd{ and } \phi^{\prime \prime}$'s coefficient is 0 whatever \textit{t} value. Therefore we have equations
  \begin{align*}
    \begin{cases}
      \alpha^{\prime \prime} + \frac{n-1}{r} \alpha^\prime = 0 \\
      - 2\alpha^\prime \beta^\prime - \frac{n-1}{r} \alpha \beta^{\prime} - \alpha \beta^{\prime \prime} = 0 \\
      \alpha ({(\beta^\prime)}^2 - 1) = 0 
    \end{cases}
  \end{align*}
  The third equation implies that $\beta = \pm x + c$ or $\alpha = 0$, which is meanless. \textit{c} is a constant value. Others two equations can be translate to
  \begin{align*}
    \begin{cases}
      p(p-1) + p(n-1) = 0 \\
      2p + n-1 = 0
    \end{cases}
  \end{align*}
  Here \textit{p} comes from $\alpha = C r^p$. The equations solution is $p = 0, -1$ correspond $n = 1, 3$.So $\alpha = C r , C r^3$. 
\end{solution}

\begin{exc}
  21.
  \begin{enumerate} [(a)]
  \item Assume $\mathbf{E} = (E^1, E^2, E^3) \text{ and } \mathbf{B} = (B^1, B^2, B^3)$ solve Maxwell's equations
    \begin{align}
      \begin{cases}
        \mathbf{E}_t = \mathrm{curl} \, \mathbf{B}, \ \mathbf{B}_t = - \mathrm{curl} \, \mathbf{E} \\
        \mathrm{div} \, \mathbf{B} = \mathrm{div} \, \mathbf{E} = 0
      \end{cases}
    \end{align}
    Show
    \begin{equation*}
      \mathbf{E}_{tt} - \Delta \mathbf{E} = 0, \quad \mathbf{B}_{tt} - \Delta \mathbf{B} = 0.
    \end{equation*}

  \item Assume that $\mathbf{u} = (u^1, u^2, u^3)$ solves the evolution equations of linear elasticity 
    \begin{equation}
      \label{eq:4}
      \mathbf{u}_{tt} - \mu \Delta \mathbf{u} - (\lambda + \mu) D(\mathrm{div}\, \mathbf{u}) = \mathbf{0} \quad \textmd{ in } \mathbb{R}^3 \times (0, \infty). 
    \end{equation}
    Show $w := \textmd{div } \mathbf{u}$ and $\mathbf{w} := \textmd{curl } \mathbf{u}$ each solve wave equations, but with differing speeds of propagation.
  \end{enumerate}
\end{exc}

\begin{solution}
  \begin{enumerate} [(a)]
  \item $\textmd{div } \mathbf{E} = 0 \Longleftrightarrow E^1_1 + E^2_2 + E^3_3 = 0$, calculating the wave equation  
    \begin{align*}
      \mathbf{E}_{tt} = &{(\textmd{curl } \mathbf{B})}_t \\
      = &{(B^3_2 - B^2_3, B^1_3 - B^3_1, B^2_1 - B^1_2)}_t \\
      = &({(- E^2_1 + E^1_2)}_2 - {(- E^1_3 + E^3_1)}_3,  \\
                        &\ {(- E^3_2 + E^2_3)}_3 - {(- E^2_1 + E^1_2)}_1,  \\
                        &\ {(- E^1_3 + E^3_1)}_1 - {(- E^3_2 + E^2_3)}_2)  \\
      = &(E^1_{11} + E^1_{22} + E^1_{33} - {(E^1_1 + E^2_2 + E^3_3)}_1,  \\
                        & E^2_{11} + E^2_{22} + E^2_{33} - {(E^1_1 + E^2_2 + E^3_3)}_2,  \\
                        & E^3_{11} + E^3_{22} + E^3_{33} - {(E^1_1 + E^2_2 + E^3_3)}_3)  \\
      = & \Delta (E^1, E^2, E^3) = \Delta \mathbf{E}.
    \end{align*}
    Similarly, get $\mathbf{B}_{tt} - \Delta \mathbf{B} = 0$.

  \item
    \begin{align*}
      w_{tt} &= \mu \textmd{div } (\textmd{div } (\textmd{gred } \mathbf{u})) + (\lambda + \mu)\textmd{div } (\textmd{gred }\mathbf{(\textmd{div } u)})  \\
             &= (\lambda + 2\mu) (\Delta (\textmd{div } \mathbf{u})) \\
             &= (\lambda + 2\mu) ( \Delta w)
    \end{align*}
  \end{enumerate}
\end{solution}

\begin{exc}
  22.  Let \textit{u} denote the density of particles moving to the right with speed one slong the real line and let \textit{v} denote the density of particles moving to the left with speed one. If at rate $d > 0$ right-moving, and vice versa, we have the system of PDE
  \begin{equation}
    \label{eq:5}
    \begin{cases}
      u_t + u_x = d(v - u) \\
      v_t - v_x = d(u - v).
    \end{cases}
  \end{equation}
  Show that both $w := u \textmd{ and } w := v$ solve the telegraph equation
  \begin{equation}
    \label{eq:6}
    w_{tt} + 2d w_t - w_{xx} = 0.
  \end{equation}
\end{exc}

\begin{solution}
  \begin{align*}
    u_{xx} &= {(d(v - u) - u_t)}_x \\
           &= d v_x - d u_x - u_{xt} \\
           &= d(- d(u - v) + v_t) - d(d(v - u) - u_t) - {(d(v - u) - u_t)}_t \\
           &= - d^2 u + d^2 v + d v_t - d^2 v + d^2 u + d u_t - d v_t + d u_t + u_{tt} \\
           &= 2d u_t + u_{tt} .
  \end{align*}
  So $w:= u$ solves the telegraph equation. $w := v$ is similar.
\end{solution}

\begin{exc}
  24.  (Equipartition of energy) Let \textit{u} solve the initial-value problem for the wave equation in one dimension:
  \begin{align}
    \begin{cases}
      u_{tt} - u_{xx} = 0 \qquad &\textmd{in } \mathbb{R} \times (0, \infty) \\
      u = g,\ u_t = h \qquad   &\textmd{on } \mathbb{R} \times \{t = 0\}.
    \end{cases}
  \end{align}
  suppose \textit{g,h} have compact support. The \textit{kinetic energy} is $k(t) := \frac{1}{2} \int_{- \infty}^{\infty} u_t^2(x,t) dx$ and the \textit{potential energy} is $p(t) := \frac{1}{2} \int_{-\infty}^{\infty} u_x^2(x,t) dx$.

  Prove
  \begin{enumerate} [(a)]
  \item $k(t) + p(t)$ is constant in \textit{t},
  \item $k(t) = p(t)$ for all large enough times \textit{t}.
  \end{enumerate}
\end{exc}

\begin{solution}
  \begin{enumerate} [(a)]
  \item Let $f(t) = k(t) + p(t)$. Differential \textit{f} with \textit{t}
    \begin{align*}
      \partial_t f &= \frac{1}{2}{\int^{\infty}_{-\infty} 2u_x u_{xt} + 2u_t u_{tt} dx} \\
                   &= \frac{1}{2} \int^{\infty}_{\infty} u_t(- u_{xx} + u_{tt})dx \\
                   &= 0.
    \end{align*}
    The second step comes from that \textit{g,h} have compact support and Finite propagation speed. So \textit{f} is constant function for \textit{t}.

  \item From d'Alembert's rule $u(x,t) = \frac{1}{2}(g(x+t) + g(x-t)) + \int_{x-t}^{x+t} h(y)dy$.
    calculate $k(t) - p(t)$
    \begin{align*}
      &k(t) - p(t) \\
      &=\frac{1}{2}\int_{-\infty}^{\infty} {(g^\prime(x+t) + g^\prime(x-t) + h(x+t) - h(x-t))}^2 \\
      &- {(g^\prime(x+t) - g^\prime(x-t) + h(x+t) + h(x-t))}^2 dx \\
      &=\frac{1}{2}\int_{-\infty}^{\infty} (2 g^\prime(x-t) - 2 h(x-t)) (2 g^\prime(x+t) - 2 h(x+t)) \\
    \end{align*}
    Since \textit{g,h} have compact support, $g^\prime, h$ have compact support. It follows that When \textit{t} is big enough. $g^\prime(x-t) - h(x-t), g^\prime(x+t) - h(x+t)$ can't have non-zero value at same time. In summary, when \textit{t} big enough $k(t) = p(t) \forall t$.
  \end{enumerate}
\end{solution}
  % \section{1}
  % \label{sec:logic}
  % \input{sec/logic.tex}

  % \section{Ordered sets}
  % \label{sec:sets}
  % \input{sec/orderedSets.tex}

  % \section{Linear algebra}
  % \label{sec:line-algebra}
  % \input{sec/linearAlgebra.tex}


\end{multicols}


\end{document}


%%% Local Variables:
%%% mode: latex
%%% TeX-master: t
%%% End:

% LocalWords:  FPN underflows denormalized FPNs matlab eps IEEE iff
% LocalWords:  cardinality significand quadratically bijection unary
% LocalWords:  contractive bijective postcondition invertible arity
% LocalWords:  subspaces surjective injective monomials additivity
% LocalWords:  nullary Abelian abelian finitary eigenvectors adjoint
% LocalWords:  eigenvector nullspace Hermitian unitarily multiset
% LocalWords:  nonsingular nonconstant homomorphism homomorphisms
% LocalWords:  isomorphically indeterminates subfield isomorphism
% LocalWords:  nondefective diagonalizable contrapositive cofactor
% LocalWords:  submatrix nilpotent positivity orthonormal extremum
% LocalWords:  Jacobian nonsquare semidefinite nonnegative RHS LLS
% LocalWords:  roundoff closedness

%%% Local Variables:
%%% mode: latex
%%% TeX-master: t
%%% End:
