\exc Compute $\lVert D_+ D_- \rVert_h$.

\begin{solution}
    Firstly, we have 
    \begin{align*}
        \lVert D_+ D_- \rVert_h \leq
         \lVert D_+ \rVert_h \lVert D_- \rVert_h
         = \frac{4}{h^2}
    \end{align*}
    Then, let $u_j = (-1)^j$, consider
    \begin{align*}
        \lVert D_+ D_- u \rVert_h^2 
        &= \sum_j ((E - 2E_0 + E^{-1})u_j)^2 / h^4 \\
        &= \sum_j 16/ h^4 = \sum_j 16/ h^4 \lVert u \rVert_h^2
    \end{align*}.
    That means 
    \[\lVert D_+ D_- \rVert_h \geq
     \sqrt{\frac{\lVert D_+ D_- u \rVert_h^2 }
     { \lVert u \rVert_h^2}} = \frac{2}{h^2} \].
    In summary, $\lVert D_+ D_- \rVert_h = \frac{2}{h^2}$. 
\end{solution}