\exc Derive estimates for 
 \[ \left| \left( D - \frac{\partial^3}{\partial x^3}\right)
 e^{i\omega x}  \right| \].
 where $ D = D^3_+, D_-D_+^2, D_-^2 D_+, D_0D_+D_-$.

 \begin{solution}
    By 
\begin{align*}
    &E^3 e^{i\omega x} = (1 + 3i\omega h - \frac{9}{2}\omega^2h^2 - 
    \frac{27}{6}i \omega^3h^3 + \frac{81}{24} \omega^4h^4 +
     \mathcal{O}(\omega^4 h^4)) e^{i\omega x} \\
    &E^2 e^{i\omega x} = (1 + 2i\omega h - \frac{4}{2}\omega^2h^2 - 
    \frac{8}{6}i \omega^3h^3 + \frac{16}{24} \omega^4h^4 +
     \mathcal{O}(\omega^4 h^4))  e^{i\omega x} \\
    &E e^{i\omega x} = (1 + i\omega h - \frac{1}{2}i\omega2h^2 - 
    \frac{1}{6}i \omega^3h^3 + \frac{1}{24} \omega^4h^4 
     \mathcal{O}(\omega^4 h^4))  e^{i\omega x} \\
    &E^{-1} e^{i\omega x} = (1 - i\omega h - \frac{1}{2}i\omega2h^2 + 
     \frac{1}{6}i \omega^3h^3 + \frac{1}{24} \omega^4h^4 
      \mathcal{O}(\omega^4 h^4))  e^{i\omega x} \\
    &E^{-2} e^{i\omega x} = (1 - 2i\omega h - \frac{4}{2}i\omega2h^2 + 
     \frac{8}{6}i \omega^3h^3 + \frac{16}{24} \omega^4h^4 
      \mathcal{O}(\omega^4 h^4))  e^{i\omega x} \\
    &E^3 e^{i\omega x} = (1 - 3i\omega h - \frac{9}{2}\omega^2h^2 + 
      \frac{27}{6}i \omega^3h^3 + \frac{81}{24} \omega^4h^4 +
       \mathcal{O}(\omega^4 h^4)) e^{i\omega x} \\
\end{align*}
\begin{enumerate}
    \item $D = D_+^3$ 
        \begin{align*}
            \left| \left( D_+^3 - \frac{\partial^3}{\partial x^3}\right)
            e^{i\omega x}  \right| &= 
            \left| \left( E^3 - 3E^2 + 3E - E_0 + i (\omega h)^3 \right)
            e^{i\omega x} / h^3  \right| \\
            &=\left| (\frac{3}{2} \omega^4 h^4 +
             \mathcal{O} (\omega^4 h^4) )  e^{i\omega x} \right| 
             =  \mathcal{O} (\omega^3 h^3)
        \end{align*}

        \item $D = D_- D_+^2$ 
        \begin{align*}
            \left| \left(D_- D_+^2 - \frac{\partial^3}{\partial x^3}\right)
            e^{i\omega x}  \right| &= 
            \left| \left( E^2 - 3E + 3E_0 - E^{-1} + i (\omega h)^3 \right)
            e^{i\omega x} / h^3  \right| \\
            &=\left| (\frac{1}{2} \omega^4 h^4 +
             \mathcal{O} (\omega^4 h^4) )  e^{i\omega x} \right|
             =  \mathcal{O} (\omega^3 h^3)
        \end{align*}
        
        \item $D = D_-^2 D_+$ 
        \begin{align*}
            \left| \left(D_-^2 D_+ - \frac{\partial^3}{\partial x^3}\right)
            e^{i\omega x}  \right| &= 
            \left| \left( E - 3E_0 + 3E^{-1} - E^{-2} + i (\omega h)^3 \right)
            e^{i\omega x} / h^3  \right| \\
            &=\left| (-\frac{1}{2} \omega^4 h^4 +
             \mathcal{O} (\omega^4 h^4) )  e^{i\omega x} \right|
             =  \mathcal{O} (\omega^3 h^3)
        \end{align*}

        \item $D = D_0 D_- D_+$ 
        \begin{align*}
            \left| \left(D_0 D_- D_+ - \frac{\partial^3}{\partial x^3}\right)
            e^{i\omega x}  \right| &= 
            \left| \left( E^2 - 2E + 2E^{-1} + E^{-2} + i (\omega h)^3 \right)
            e^{i\omega x} / h^3  \right| \\
            &=\left| (
            \mathcal{O} (\omega^4 h^4) )  e^{i\omega x} \right|
            =  \mathcal{O} (\omega^4 h^4)
        \end{align*}
\end{enumerate}

 \end{solution}