\documentclass[a4paper]{book}
% chktex-file 
% chktex-file 3
\usepackage{geometry}
% make full use of A4 papers
\geometry{margin=1.5cm, vmargin={0pt,1cm}}
\setlength{\topmargin}{-1cm}
\setlength{\paperheight}{29.7cm}
\setlength{\textheight}{25.1cm}

% auto adjust the marginals
\usepackage{marginfix}

\usepackage{amsfonts}
\usepackage{amsmath}
\usepackage{amssymb}
\usepackage{amsthm}
% \usepackage{CJKutf8}   % for Chinese characters
\usepackage{ctex}
\usepackage{enumerate}
\usepackage{graphicx}  % for figures
\usepackage{layout}
\usepackage{multicol}  % multiple columns to reduce number of pages
\usepackage{mathrsfs}
\usepackage{fancyhdr}
\usepackage{subfigure}
\usepackage{tcolorbox}
\usepackage{tikz-cd}
\usepackage{listings}
\usepackage{xcolor} %代码高亮
\usepackage{braket}
% ------------------
% common commands %
% ------------------
% differentiation
\newcommand{\gen}[1]{\left\langle#1 \right\rangle}
\newcommand{\dif}{\mathrm{d}}
\newcommand{\difPx}[1]{\frac{\partial#1}{\partial x}}
\newcommand{\difPy}[1]{\frac{\partial#1}{\partial y}}
\newcommand{\Dim}{\mathrm{D}}
\newcommand{\avg}[1]{\left\langle#1 \right\rangle}
\newcommand{\sgn}{\mathrm{sgn}}
\newcommand{\Span}{\mathrm{span}}
\newcommand{\dom}{\mathrm{dom}}
\newcommand{\Arity}{\mathrm{arity}}
\newcommand{\Int}{\mathrm{Int}}
\newcommand{\Ext}{\mathrm{Ext}}
\newcommand{\Cl}{\mathrm{Cl}}
\newcommand{\Fr}{\mathrm{Fr}}
% group is generated by
\newcommand{\grb}[1]{\left\langle#1 \right\rangle}
% rank
\newcommand{\rank}{\mathrm{rank}}
\newcommand{\Iden}{\mathrm{Id}}

% this environment is for solutions of examples and exercises
\newenvironment{solution}%
{\noindent\textbf{Solution.}}%
{\qedhere}
% the following command is for disabling environments
% so that their contents do not show up in the pdf.
\makeatletter
\newcommand{\voidenvironment}[1]{%
  \expandafter\providecommand\csname env@#1@save@env\endcsname{}%
  \expandafter\providecommand\csname env@#1@process\endcsname{}%
  \@ifundefined{#1}{}{\RenewEnviron{#1}{}}%
}
\makeatother

% ---------------------------------------------
% commands specifically for complex analysis %
% ---------------------------------------------
% complex conjugate
\newcommand{\ccg}[1]{\overline{#1}}
% the imaginary unit
\newcommand{\ii}{\mathbf{i}}
% \newcommand{\ii}{\boldsymbol{i}}
% the real part
\newcommand{\Rez}{\mathrm{Re}\,}
% the imaginary part
\newcommand{\Imz}{\mathrm{Im}\,}
% punctured complex plane
\newcommand{\pcp}{\mathbb{C}^{\bullet}}
% the principle branch of the logarithm
\newcommand{\Log}{\mathrm{Log}}
% the principle value of a nonzero complex number
\newcommand{\Arg}{\mathrm{Arg}}
\newcommand{\Null}{\mathrm{null}}
\newcommand{\Range}{\mathrm{range}}
\newcommand{\Ker}{\mathrm{ker}}
\newcommand{\Iso}{\mathrm{Iso}}
\newcommand{\Aut}{\mathrm{Aut}}
\newcommand{\ord}{\mathrm{ord}}
\newcommand{\Res}{\mathrm{Res}}
% \newcommand{\GL2R}{\mathrm{GL}(2,\mathbb{R})}
\newcommand{\GL}{\mathrm{GL}}
\newcommand{\SL}{\mathrm{SL}}
\newcommand{\Dist}[2]{\left|{#1}-{#2}\right|}

\newcommand\tbbint{{-\mkern-16mu\int}}
\newcommand\tbint{{\mathchar'26 -\mkern-14mu\int}}
\newcommand\dbbint{{-\mkern-20mu\int}}
\newcommand\dbint{{\mathchar'26 -\mkern-26mu\int}}
\newcommand\bint{
  {\mathchoice{\dbint}{\tbint}{\tbint}{\tbint}}
}
\newcommand\bbint{
  {\mathchoice{\dbbint}{\tbbint}{\tbbint}{\tbbint}}
}





% ----------------------------------------
% theorem and theorem-like environments %
% ----------------------------------------
\numberwithin{equation}{chapter}
\theoremstyle{definition}

\newtheorem{thm}{Theorem}[chapter]
\newtheorem{axm}[thm]{Axiom}
\newtheorem{alg}[thm]{Algorithm}
\newtheorem{asm}[thm]{Assumption}
\newtheorem{defn}[thm]{Definition}
\newtheorem{prop}[thm]{Proposition}
\newtheorem{rul}[thm]{Rule}
\newtheorem{coro}[thm]{Corollary}
\newtheorem{lem}[thm]{Lemma}
\newtheorem{exm}{Example}[chapter]
\newtheorem{rem}{Remark}[chapter]
\newtheorem{exc}[exm]{Exercise}
\newtheorem{frm}[thm]{Formula}
\newtheorem{ntn}{Notation}

% for complying with the convention in the textbook
\newtheorem{rmk}[thm]{Remark}


% \lstset{
%	backgroundcolor=\color{red!50!green!50!blue!50},%代码块背景色为浅灰色
%	rulesepcolor= \color{gray}, %代码块边框颜色
%	breaklines=true,  %代码过长则换行
%	numbers=left, %行号在左侧显示
%	numberstyle= \small,%行号字体
%	keywordstyle= \color{blue},%关键字颜色
%	commentstyle=\color{gray}, %注释颜色
%	frame=shadowbox%用方框框住代码块
% }
\lstset{
  columns=fixed,
  numbers=left,                                        % 在左侧显示行号
  numberstyle=\tiny\color{gray},                       % 设定行号格式
  frame=none,                                          % 不显示背景边框
  backgroundcolor=\color[RGB]{245,245,244},            % 设定背景颜色
  keywordstyle=\color[RGB]{40,40,255},                 % 设定关键字颜色
  numberstyle=\footnotesize\color{darkgray},
  commentstyle=\it\color[RGB]{0,96,96},                % 设置代码注释的格式
  stringstyle=\rmfamily\slshape\color[RGB]{128,0,0},   % 设置字符串格式
  showstringspaces=false,                              % 不显示字符串中的空格
  language=c++,                                        % 设置语言
}

% ----------------------
% the end of preamble %
% ----------------------

\begin{document}
\pagestyle{empty}
\pagenumbering{roman}
% 
% \tableofcontents
% \clearpage

% \pagestyle{fancy}
% \fancyhead{}
% \lhead{Qinghai Zhang}
% \chead{Notes on Algebraic Topology}
% \rhead{Fall 2018}


\setcounter{chapter}{7}
\pagenumbering{arabic}
% \setcounter{page}{0}

% --------------------------------------------------------
% uncomment the following to remove these environments
% to generate handouts for students.
% --------------------------------------------------------
% \begingroup
% \voidenvironment{rem}%
% \voidenvironment{proof}%
% \voidenvironment{solution}%


% each chapter is factored into a separate file.

\chapter{Homework 21935004 谭焱}
% \begin{lstlisting}
%   int main(){
%   double d;
%   int i;
%   return i;
% }
% \end{lstlisting}
% The main ingredients of snacks are sugar and fat;
% the main ingredients of math are logic and set theory.


% \begin{multicols}{2}
%   \setlength{\columnseprule}{0.2pt}

\begin{exc}
  15.  Assuming %$H \colon \mathbb{R}^n \rightarrow \mathbb{R}$ is uniformly convex and
  \[H(\frac{p_1 + p_2}{2}) \leq \frac{1}{2}H(p_1) + \frac{1}{2}H(p_2) - \frac{\theta}{8}\left| p_1 - p_2 \right|^2.\]
  Prove
  \[\frac{1}{2}L(q_1) + \frac{1}{2}L(q_2) \leq L(\frac{q_1 + q_2}{2}) + \frac{1}{8 \theta} \left| q_1 - q_2 \right|^2.\]
\end{exc}

\begin{solution}
  From the definition of $L$, Let $L(q_1) = \max\limits_{p \in \mathbb{R}^n}\{q_1 \cdot p - H(p)\} = q_1 \cdot p_1 - H(p_1), L(q_2) = q_2 \cdot p_2 - H(p_2)$. Then
  \begin{align*}
    \frac{1}{2}L(q_1) + \frac{1}{2}L(q_2) &\leq L(\frac{q_1 + q_2}{2}) + \frac{1}{8 \theta} \left| q_1 - q_2 \right|^2  \Longleftrightarrow \\
    \frac{1}{2}(p_1q_1 + p_2q_2) + H(\frac{p_1 + p_2}{2}) &\leq \frac{1}{2}H(p_1) + \frac{1}{2}H(p_2) + \frac{1}{4}(p_1q_1 + p_1q_2 + p_2q_1 + p_2q_2) +  \frac{1}{8 \theta} \left| q_1 - q_2 \right|^2 \Longleftarrow \\
    \frac{1}{4}(p_1 - p_2)(q_1 - q_2) &\leq \frac{\theta}{8}\left| p_1 - p_2 \right|^2 + \frac{1}{8 \theta} \left| q_1 - q_2 \right|^2 \Longrightarrow \\
    \frac{1}{4}(p_1 - p_2)(q_1 - q_2) &\leq 2 \sqrt\left({\frac{\theta}{8}\left| {p_1 - p_2} \right|^2 \times \frac{1}{8 \theta} \left| {q_1 - q_2} \right|^2} \right).
  \end{align*}
  The last equation is obvious.
\end{solution}


\begin{exc}
  17.  Show that
  \begin{equation*}
    u(x,t) :=
    \begin{cases}
      \begin{aligned}
      - \frac{2}{3}\left( t + \sqrt{3x + t^2} \right)& \qquad \textmd{if } 4x + t^2 > 0 \\
      0& \qquad \textmd{if } 4x + t^2 < 0
      \end{aligned}
    \end{cases}
  \end{equation*}
  is an (unbounded) entropy solution of $u_t + (\frac{u^2}{2})_x = 0$.
\end{exc}

\begin{solution}
  Since while $u(x,t) = 0$ the equations holds trival, and When $u(x,t) \not= 0$ 
  \begin{align*}
    u_t + \left( \frac{u^2}{2} \right)_x &= (-\frac{2}{3}t - \frac{2}{3}\sqrt{3x + t^2})_t + \left( \frac{4 }{9}t^2 + \frac{2}{3}x + \frac{4}{9}t\sqrt{3x + t^2} \right)_x \\
                                         &= - \frac{2}{3} - \frac{2t}{3\sqrt{3x + t^2}} + \frac{2}{3} + \frac{2t}{3\sqrt{3x + t^2}}\\
    &= 0
  \end{align*}
  therefore, it's a intergal solution of $u_t + (\frac{u^2}{2})_x = 0$. Then
  %assuming $u(x+z,t) \not 0, u(x,t) \not 0$, have
  \begin{align*}
    u(x + z, t) - u(x,t) =
    \begin{cases}
      \frac{2}{3}(\sqrt{3x + 3z + t^2} - \sqrt{3x + t^2} ) =\frac{2z}{\sqrt{3x + 3z + t^2} - \sqrt{3x + t^2}} \leq \frac{2}{t}z \quad &\textmd{if } x+z > x > -\frac{t^2}{4}  \\
      \frac{2}{3}(\sqrt{3x + 3z + t^2}) < 0 < z \quad &\textmd{if } x+z > -\frac{t^2}{4} > x \\
      0 < z \quad &\textmd{if } -\frac{t^2}{4} > x+z > x
    \end{cases}.
  \end{align*}
  So this is an entropy solution of $u_t + (\frac{u^2}{2})_x = 0$.
\end{solution}


\begin{exc}
  18.  Assume $u(x + z) - u(x) \leq Ez$ for all $z > 0$. Let $u^{\epsilon} = \eta_\epsilon * u$, and show
  \[u_x^\epsilon \leq E.\]
\end{exc}

\begin{solution}
  if $u_x^\epsilon > E$ while $x = x_0$, that's equal to
  \begin{align*}
    u_x^\epsilon(x_0) &= (\int_{B(0,\epsilon)}\eta_\epsilon(y)f(x_0 -y)dy)_x \\
                      &= \int_{B(0,\epsilon)}\eta_\epsilon(y)f_x(x_0 -y)dy \\
    & > E.
  \end{align*}
  It's implies that $\exist x_1 \in B(x_0,\epsilon), f_x(x_1) > E$,Or $\int_{B(0,\epsilon)}\eta_\epsilon(y)f_x(x_0 -y)dy \leq \int_{B(0,\epsilon)}\eta_\epsilon(y)Edy = E$. Which is contracdicte with $u_x^\epsilon(x_0) > E$. Since $u_x$ has to continuous, $\exist B(x_1, \epsilon), \forall x \in B(x_1, \epsilon) s.t u_x(x) > E$. Then let $z \in B(x_1, \frac{\epsilon}{2})$ so that $u(x + z) - u(x) = u_x(\zeta) z, \zeta \in B(x_1, \epsilon) \Rightarrow u(x +z) - u(x) > E *z$. It's contracdicate with $u(x + z) - u(x) \leq Ez$.
\end{solution}


\begin{exc}
  19.  Assume $F(0) = 0$, $u$ is a continuous integral solution of the conservation law
  \begin{equation*}
    \begin{cases}
      \begin{aligned}
        u_t + F(u)_x = 0 \qquad &\textmd{in } \mathbb{R} \times (0, \infty) \\
        u = g \qquad &\textmd{on } \mathbb{R} \times \{t = 0\}.
      \end{aligned}
    \end{cases}
  \end{equation*}
  and $u$ has compact support in $\mathbb{R} \times [0, T]$ for each time $T > 0$. Prove
  \[\int_{-\infty}^{\infty} u(\cdot,t)dx = \int_{-\infty}^{\infty}g dx\]
  for all $t > 0$.
\end{exc}

\begin{solution}
  Derivate left get
  \begin{align*}
    \frac{d}{dt}(\int_{-\infty}^{\infty}u(\cdot,t)dx) &= \int_{-\infty}^{\infty}u_t(\cdot,t)dx \\
                                                      &= \int_{-\infty}^{\infty}\frac{d}{dx}(F(u))dx \\
                                                      &= \left. F(u) \right|_{-\infty}^\infty \\
                                                      &= 0
  \end{align*}
  The last step from $u$ has compact support and $F(0) = 0$. And it indicate $\int_{-\infty}^{\infty} u(\cdot,t)dx = \int_{-\infty}^{\infty} u(\cdot,0)dx = \int_{-\infty}^{\infty} gdx$.
\end{solution}

\begin{exc}
  20.  Compute explicitly the unique entropy solution of
  \begin{equation*}
    \begin{cases}
      \begin{aligned}
        u_t + \left( \frac{u^2}{2} \right)_x = 0 \qquad& \textmd{in } \mathbb{R} \times (0, \infty) \\
        u = g \qquad& \textmd{on } \mathbb{R} \times \{t = 0\},
      \end{aligned}
    \end{cases}
  \end{equation*}
  for
  \begin{equation*}
    g(x) = 
    \begin{cases}
      \begin{aligned}
        1 & \qquad \textmd{if } x < -1 \\
        0 & \qquad \textmd{if } -1 < x < 0 \\
        2 & \qquad \textmd{if } 0 < x < 1 \\
        0 & \qquad \textmd{if } 1 < x.
      \end{aligned}
    \end{cases}
  \end{equation*}
  Draw a picture documenting your answer, being sure to illustrate what happens for all times $ t > 0$.
\end{exc}

\begin{solution}
  %Solve the characteristic equations get the solution $u$ will be constant value $z^0 = g(x^0)$ along the projected characteristic
  %\[\mathbf{y}(s) = (g(x^0)s + x^0,s) (s \geq 0)\]
  %for each $x^0 \in \mathbb{R}$.
  Solve the equations
  \begin{align*}
    \begin{cases}
      w_t + \frac{w_x^2}{2} = 0 \qquad& \textmd{in } \mathbb{R} \times (0, \infty) \\
      w = \int_0^x g(s)ds \qquad& \textmd{on } \mathbb{R} \times \{t = 0\},
    \end{cases}
  \end{align*}
  get $w(x, t) = \min\limits_{y \in \mathbb{R}}{t\frac{(x - y)^2}{2t^2} +\int_0^y g(s)ds}$.Let $f(y)= \frac{d}{dy}(t\frac{(x - y)^2}{2t^2} + \int_0^y g(s)ds ) = -\frac{(x - y)}{t} + g(y)$, Therefore, discussing by situation
  \begin{enumerate}
  \item $x < -1$
    \[f(y) =
      \begin{aligned}
      \begin{cases}
        > 0 \qquad &\textmd{if } y > x-t \\
        =0   \qquad &\textmd{if } y = x-t \\
        < 0  \qquad &\textmd{if } y < x-t \\
      \end{cases}
      \end{aligned}
    \]
    \[w(x,t) = \frac{t}{2} + \int_0^{x-t} g(s)ds \Rightarrow u(x,t) = 1 .\]

  \item $-1 < x < 0$
    \[f(y) =
      \begin{aligned}
        \begin{cases}
         \begin{cases}
          > 0 \qquad &\textmd{if } y > x \\
          = 0   \qquad &\textmd{if } y = x \\
          < 0  \qquad &\textmd{if } y < x \\
        \end{cases}  \qquad &\textmd{if } t < 2 * (x+1)\\
        \begin{cases}
          > 0 \qquad &\textmd{if } y > x-t \\
          = 0   \qquad &\textmd{if } y = x-t \\
          < 0  \qquad &\textmd{if } y < x-t \\
        \end{cases}  \qquad &\textmd{if } t > 2 * (x+1)
        \end{cases}
      \end{aligned}
    \]
    \[w(x,t) =
      \begin{cases}
        \int_0^{x} g(s)ds \Rightarrow u(x,t)  = 0  \Rightarrow u(x,t) = g(x) = 0 \qquad &\textmd{if } t < 2 * (x+1) \\
        \frac{t}{2} + \int_0^{x-t} g(s)ds  \Rightarrow u(x,t) = g(x-t) = 1  \qquad &\textmd{if } t > 2 * (x+1) \\
      \end{cases}
    \]

  \item $0 < x < 1$
    \[f(y) =
      \begin{aligned}
        \begin{cases}
          \begin{cases}
            > 0 \qquad &\textmd{if } x - t < y < 0\ ||\ 0 < y \\
            %= 0   \qquad &\textmd{if } y = 0 \\
            < 0  \qquad &\textmd{if } y < x - t \\
          \end{cases}  \qquad &\textmd{if } x < t - (2t)^{1/2} \\
          \begin{cases}
            > 0 \qquad &\textmd{if } x - t < y < 0 \ ||\ 0 < y \\
            %= 0   \qquad &\textmd{if } y = x-t \\
            < 0  \qquad &\textmd{if } y < x - t \\
          \end{cases}  \qquad &\textmd{if } t - (2t)^{1/2} < x < 2t \\
          \begin{cases}
            > 0 \qquad &\textmd{if } x - t < y < -1\ ||\ x - 2t < y \\
            % = 0   \qquad &\textmd{if } y = x-t \\
            < 0  \qquad &\textmd{if } y < x - t\ ||\ -1 < y < x - 2t \\
          \end{cases}  \qquad &\textmd{if } 2t < x \\
        \end{cases}
      \end{aligned}
    \]
    \[w(x,t) =
      \begin{cases}
        \min\{\frac{t}{2} + \int_0^{x-t} g(s)ds, \frac{x^2}{2t} + \int_0^{0} g(s)ds\} = \frac{t}{2} + \int_0^{x-t} g(s)ds \\ \Rightarrow u(x,t)  = g(x-t),(x - t) < -2  \Rightarrow u(x,t) = 1 \qquad &\textmd{if } x < t - (2t)^{1/2} \\
        \min\{\frac{t}{2} + \int_0^{x-t} g(s)ds, \frac{x^2}{2t} + \int_0^{0} g(s)ds\} = \frac{x^2}{2t} + \int_0^{0} g(s)ds \\ \Rightarrow u(x,t) = \frac{x}{t} + g(0) = \frac{x}{t}  \qquad &\textmd{if } t - (2t)^{1/2} < x < 2t \\
        \min\{\frac{t}{2} + \int_0^{x-t} g(s)ds, 2t + \int_0^{x-2t} g(s)ds\} = 2t + \int_0^{x-2t} g(s)ds \\ \Rightarrow u(x,t) = g(x-2t) = 2  \qquad &\textmd{if } 2t < x \\
      \end{cases}
    \]

  \item $1 < x < 4 + 2\sqrt{2}$
    \[f(y) =
      \begin{aligned}
        \begin{cases}
          \begin{cases}
            > 0 \qquad &\textmd{if } x - t < y < -1\ ||\ 0 < y < 1\ || \ x < y \\
            % = 0   \qquad &\textmd{if } y = 0 \\
            < 0  \qquad &\textmd{if } y < x - t\ ||\ -1 < y < 0 \ || \ 1 < y < x \\
          \end{cases}  \qquad &\textmd{if } x < t - (2t)^{1/2} \\
          \begin{cases}
            > 0 \qquad &\textmd{if } (x - t < y < 0) \\&(\textmd{maybe} x-t < -1\textmd{but no influence to anwser})\\ &\ ||\ 0 < y < 1 \ ||\ x < y  \\
            % = 0   \qquad &\textmd{if } y = x-t \\
            < 0  \qquad &\textmd{if } y < x - t \ || \1 < y < x \\
          \end{cases}  \qquad &\textmd{if } t - (2t)^{1/2} < x < 2t \&\& x < 2t^{1/2}   \\
          \begin{cases}
            > 0 \qquad &\textmd{if } y < 0\ ||\ x - 2t < y \\
            % = 0   \qquad &\textmd{if } y = x-t \\
            < 0  \qquad &\textmd{if } y < x - t\ ||\ -1 < y < x - 2t \\
          \end{cases}  \qquad &\textmd{if } 2t < x < 1 + t \\
          \begin{cases}
            > 0 \qquad &\textmd{if } y < 1 \ || \ x < y \\
            % = 0   \qquad &\textmd{if } y = x-t \\
            < 0  \qquad &\textmd{if } x < y  \\
          \end{cases}  \qquad &\textmd{if } (2t^{1/2} < y \&\& t < 1) \ ||\\& \ ( 2t < y \&\& t > 1)
        \end{cases}
      \end{aligned}
    \]
    \[w(x,t) =
      \begin{cases}
        \min\{\frac{t}{2} + \int_0^{x-t} g(s)ds, \frac{x^2}{2t} + \int_0^{0} g(s)ds, \int_0^{x} g(s)ds\} = \frac{t}{2} + \int_0^{x-t} g(s)ds \\ \Rightarrow u(x,t)  = g(x-t),(x - t) < -1  \Rightarrow u(x,t) = 1 \qquad &\textmd{if } x < t - (2t)^{1/2} \\
        \min\{\frac{t}{2} + \int_0^{x-t} g(s)ds, \frac{x^2}{2t} + \int_0^{0} g(s)ds, \int_0^{x} g(s)ds \} = \frac{x^2}{2t} + \int_0^{0} g(s)ds \\\Rightarrow u(x,t) = \frac{x}{t} + g(0) = \frac{x}{t}  \qquad &\textmd{if }  t - (2t)^{1/2} < x < 2t \&\&\\ &x < 2t^{1/2} \\
        \min\{\frac{t}{2} + \int_0^{x-t} g(s)ds, 2t + \int_0^{x-2t} g(s)ds\} = 2t + \int_0^{x-2t} g(s)ds \\ \Rightarrow u(x,t) = g(x-2t) = 2  \qquad &\textmd{if } 2t < x < 1 + t \\
        \min\{\int_0^{x} g(s)ds\} = \int_0^{x} g(s)ds \\ \Rightarrow u(x,t) = g(x) = 0  \qquad &\textmd{if }  t < x.
      \end{cases}
    \]

  \item  $4 + 2\sqrt{2} < x$
    \[u(x,t) =
      \begin{aligned}
        \begin{cases}
          1 \qquad & \textmd{if } 2x -2 < t \\
          0 \qquad & \textmd{if } t < 2x -2  \\
        \end{cases}
      \end{aligned}
    \]
  \end{enumerate}

  In summary,
  \begin{align*}
    u(x,t) =
    \begin{cases}
      1   \qquad & \textmd{if }  x < 0\ \&\& \ 2x + 2 < t \\
      0   \qquad & \textmd{if }  x < 0\ \&\& \ t < 2x + 2 \\
      1   \qquad & \textmd{if }  0 < x < 4 + 2\sqrt{2} \ \&\& \ x < t - \sqrt{2t} \\
      2   \qquad & \textmd{if }  0 < x < 2  \ \&\& \ x - 1 < t < \frac{1}{2}x \\
      \frac{x}{t}  \qquad & \textmd{if }  0 < x < 4 + 2\sqrt{2} \ \&\& \ t -  \sqrt{2t} < x \\
      & \ \&\& \  \frac{1}{2} < t \textmd{ while } 0 < x \leq 2 \ \&\& \ \frac{1}{4}x^2 < t \textmd{ while } 2 < x < 4 + 2\sqrt{2} \\
      1   \qquad & \textmd{if }  4 + 2\sqrt{2} < x \ \&\& \ 2x - 2 < t \\
      0   &\textmd{otherwise}.
    \end{cases}
  \end{align*}.
  And $u(x,t)$ plot in (\ref{fig:1})
  \begin{figure}}\label{fig:1}
    \centering
    \includegraphics[scale = 0.25]{u}
    \caption{$u(x,t)$}
  \end{figure}
\end{solution}





%   \section{1}
%   \label{sec:logic}
%   \input{sec/logic.tex}

%   \section{Ordered sets}
%   \label{sec:sets}
%   \input{sec/orderedSets.tex}

%   \section{Linear algebra}
%   \label{sec:line-algebra}
%   \input{sec/linearAlgebra.tex}


% \end{multicols}


\end{document}


%%% Local Variables:
%%% mode: latex
%%% TeX-master: t
%%% End:

% LocalWords:  FPN underflows denormalized FPNs matlab eps IEEE iff
% LocalWords:  cardinality significand quadratically bijection unary
% LocalWords:  contractive bijective postcondition invertible arity
% LocalWords:  subspaces surjective injective monomials additivity
% LocalWords:  nullary Abelian abelian finitary eigenvectors adjoint
% LocalWords:  eigenvector nullspace Hermitian unitarily multiset
% LocalWords:  nonsingular nonconstant homomorphism homomorphisms
% LocalWords:  isomorphically indeterminates subfield isomorphism
% LocalWords:  nondefective diagonalizable contrapositive cofactor
% LocalWords:  submatrix nilpotent positivity orthonormal extremum
% LocalWords:  Jacobian nonsquare semidefinite nonnegative RHS LLS
% LocalWords:  roundoff closedness

%%% Local Variables:
%%% mode: latex
%%% TeX-master: t
%%% End:
